byteback-whyml/src/main/java/byteback/mlcfg/syntax/expr/InstanceOfExpression.java
@@ -1,0 +1,35 @@
+package byteback.mlcfg.syntax.expr;
+
+import byteback.mlcfg.syntax.types.WhyJVMType;
+import byteback.mlcfg.syntax.types.WhyType;
+
+public class InstanceOfExpression implements Expression {
+	private final Expression reference;
+	private final WhyType type;
+
+	public InstanceOfExpression(Expression reference, WhyType type) {
+		if (reference.type() != WhyJVMType.PTR) {
+			throw new IllegalArgumentException("instanceof expression must have type PTR, given " + reference.type());
+		}
+
+		if (type.jvm() != WhyJVMType.PTR) {
+			throw new IllegalArgumentException("instanceof type to check must have JVM type PTR, given " + type.jvm());
+		}
+
+		this.reference = reference;
+		this.type = type;
+	}
+
+	@Override
+	public String toWhy() {
+		return "(checkcast heap (%s) (%s))".formatted(
+				reference.toWhy(),
+				type.getPreludeType()
+		);
+	}
+
+	@Override
+	public WhyJVMType type() {
+		return WhyJVMType.PTR;
+	}
+}
