byteback-whyml/src/main/java/byteback/mlcfg/syntax/expr/QuantifierExpression.java
@@ -1,0 +1,66 @@
+package byteback.mlcfg.syntax.expr;
+
+import byteback.mlcfg.syntax.WhyFunctionParam;
+import byteback.mlcfg.syntax.types.WhyJVMType;
+import java.util.List;
+import java.util.Optional;
+import java.util.stream.Collectors;
+
+public class QuantifierExpression implements Expression {
+	private final Kind kind;
+	private final List<WhyFunctionParam> variableList;
+	private final Expression inner;
+
+	public QuantifierExpression(Kind kind, List<WhyFunctionParam> variableList, Expression inner) {
+		if (variableList.isEmpty()) {
+			throw new IllegalArgumentException("quantifier must have one or more variables");
+		}
+
+		this.kind = kind;
+		this.variableList = variableList;
+		this.inner = inner;
+	}
+
+	@Override
+	public String toWhy() {
+		final String whyVarList = variableList.stream()
+				.map(e -> "%s: %s".formatted(e.name(), e.type().getWhyType()))
+				.collect(Collectors.joining(", "));
+
+		final String conditionList = variableList.stream()
+				.map(WhyFunctionParam::condition)
+				.flatMap(Optional::stream)
+				.collect(Collectors.joining(" && "));
+
+		if (conditionList.isEmpty()) {
+			return "(%s %s. (%s))".formatted(
+					kind.symbol,
+					whyVarList,
+					inner.toWhy()
+			);
+		} else {
+			return "(%s %s. (%s) -> (%s))".formatted(
+					kind.symbol,
+					whyVarList,
+					conditionList,
+					inner.toWhy()
+			);
+		}
+	}
+
+	@Override
+	public WhyJVMType type() {
+		return WhyJVMType.BOOL;
+	}
+
+	public enum Kind {
+		EXISTS("exists"),
+		FORALL("forall");
+
+		private final String symbol;
+
+		Kind(String symbol) {
+			this.symbol = symbol;
+		}
+	}
+}
