byteback-whyml/src/main/java/byteback/mlcfg/syntax/expr/StringLiteralExpression.java
@@ -1,0 +1,47 @@
+package byteback.mlcfg.syntax.expr;
+
+import byteback.mlcfg.syntax.types.WhyJVMType;
+import com.google.common.base.Charsets;
+
+public class StringLiteralExpression implements Expression {
+	private final String str;
+
+	public StringLiteralExpression(String str) {
+		this.str = str;
+	}
+
+	private static String mapChar(byte c) {
+		if ((c >= '0' && c <= '9') || (c >= 'A' && c <= 'Z') || c >= 'a' && c <= 'z') {
+			return Character.toString(c);
+		} else if (c == '\\') {
+			return "\\\\";
+		} else if (c == '"') {
+			return "\\\"";
+		} else if (c == '\n') {
+			return "\\n";
+		} else if (c == '\r') {
+			return "\\r";
+		} else if (c == '\t') {
+			return "\\t";
+		} else {
+			return "\\x%02X".formatted((int) c & 0xff);
+		}
+	}
+
+	@Override
+	public String toWhy() {
+		final StringBuilder sb = new StringBuilder("\"");
+		for (final byte b : str.getBytes(Charsets.UTF_8)) {
+			sb.append(mapChar(b));
+		}
+		sb.append("\"");
+
+		final String literal = sb.toString();
+		return "(java.lang.String.literal'8 heap %s)".formatted(literal);
+	}
+
+	@Override
+	public WhyJVMType type() {
+		return WhyJVMType.PTR;
+	}
+}
