byteback-frontend/boogie/src/test/resources/boogie/Simple.bpl
@@ -1,4 +1,4 @@
-type Unit;
+kind Unit;
 
 const unique unit : Unit;
 
